theories/L/AbstractMachines/FlatPro/UnfoldHeap.v
@@ -1,0 +1,280 @@
+From Undecidability.L.AbstractMachines.FlatPro Require Import LM_heap_correct LM_heap_def.
+From Undecidability.L.Prelim Require Import LoopSum.
+
+Set Default Proof Using "Type".
+Section fixH.
+  Variable H : Heap.
+
+  (** We define a function to unfold a closure, needed for the Turing machine M_unf. *)
+  (* function that unfolds if unfoldable *)
+  Definition unfoldTailRecStep '(stack,res) : (list (HClos*nat) * Pro) + option Pro :=
+  match stack with
+    | ((a,P),k)::stack =>
+      match P with
+        c::P =>
+          match c with
+            varT n =>
+              if ( k <=? n)
+              then
+                  match lookup H a (n-k) with
+                  | Some (b,Q) =>
+                    inl (((b,Q),1)::(a,retT::P,S k)::stack,lamT::res)
+                  | None => inr None
+                  end
+              else
+                inl ((a,P,k)::stack,varT n::res)   
+          | appT => inl ((a,P,k)::stack,appT::res)         
+          | lamT => inl ((a,P,S k)::stack,lamT::res)
+          | retT => inl ((a,P,pred k)::stack,retT::res)
+          end
+        | [] => inl (stack,res)
+      end
+    | [] => inr (Some res)
+  end.
+
+  (*
+  Lemma unfoldTailRecStep_retT a k stack res fuel m:
+    loopSum ((m+1) + fuel) unfoldTailRecStep ((a,repeat retT m,k)::stack,res)
+    = loopSum fuel unfoldTailRecStep (stack,repeat retT m ++ res).
+  Proof.
+    induction m in k,res|-*;cbn. reflexivity. 
+    rewrite app_comm_cons,repeat_cons,<- app_assoc.
+    erewrite <- IHm. reflexivity.
+  Qed.
+
+  
+  Lemma unfoldTailRecStep_split_stack stack fuel:
+  exists fuel', forall stack' res,
+  loopSum fuel unfoldTailRecStep (stack++stack',res)
+  = match loopSum ((fuel-fuel') + 1) unfoldTailRecStep (stack,res) with
+      | Some res' => loopSum fuel' unfoldTailRecStep (stack',rev res')
+      | x => x
+  end /\ fuel' <= fuel.
+  Proof.
+    induction fuel in stack|-*. 
+    { exists 0. intros. destruct (loopSum (_ + 1)). all:now cbn. } 
+    destruct stack as [ | [[a [|c P]] k] stack]. 
+    - exists (S fuel). intros. rewrite Nat.sub_diag.
+      remember (S fuel) as tmp. cbn. now rewrite rev_involutive.
+    - specialize IHfuel with (stack:=stack) as (fuel'&IH). 
+      exists fuel'. intros. specialize IH as (IH&?).
+      rewrite Nat.sub_succ_l. 2:nia.
+      cbn. rewrite IH. easy.
+    - setoid_rewrite Nat.add_comm. cbn - ["-"].
+      destruct c;cbn - ["-"].
+      + destruct (Nat.leb_spec0 k n). destruct lookup as [[]|].
+        * destruct (IHfuel ((h, l0, 1) :: (a, retT :: P, S k) :: stack)) as (fuel1&IH1). cbn in IH1.
+          eexists (fuel1). intros. specialize IH1 as (->&?). 
+          rewrite Nat.sub_succ_l. rewrite Nat.add_1_r. all:easy. 
+        * destruct (IHfuel ((a, P, k) :: stack)) as (fuel1&IH1). cbn in IH1.
+          eexists (fuel1). intros. specialize IH1 as (->&?).  
+          rewrite Nat.sub_succ_l. rewrite Nat.add_1_r. all:easy.
+        * destruct (IHfuel ((a, P, k) :: stack)) as (fuel1&IH1). cbn in IH1.
+          eexists (fuel1). intros. specialize IH1 as (->&?).  
+          rewrite Nat.sub_succ_l. rewrite Nat.add_1_r. all:easy. 
+      + destruct (IHfuel ((a, P, k) :: stack)) as (fuel1&IH1). cbn in IH1.
+        eexists (fuel1). intros. specialize IH1 as (->&?).  
+        rewrite Nat.sub_succ_l. rewrite Nat.add_1_r. all:easy.
+      + destruct (IHfuel ((a, P, S k) :: stack)) as (fuel1&IH1). cbn in IH1.
+        eexists (fuel1). intros. specialize IH1 as (->&?).  
+        rewrite Nat.sub_succ_l. rewrite Nat.add_1_r. all:easy.
+      + destruct (IHfuel ((a, P, Nat.pred k) :: stack)) as (fuel1&IH1). cbn in IH1.
+        eexists (fuel1). intros. specialize IH1 as (->&?).  
+        rewrite Nat.sub_succ_l. rewrite Nat.add_1_r. all:easy.   
+  Qed.
+
+(*
+Lemma unfoldTailRecStep_splita a k s P stack res fuel:
+  loopSum fuel unfoldTailRecStep ((a,compile s++P,k)::stack,res)
+  = loopSum fuel unfoldTailRecStep ((a,compile s,k)::(a,P,k)::stack,res).
+Proof.
+  induction fuel in s,stack,res,P|-*. reflexivity.
+  destruct s;cbn.
+  - destruct (Nat.leb_spec0 k n). destruct lookup as [[]|].
+  - eexists (1). cbn [loopSum unfoldTailRecStep plus compile]. cbn. 
+    destruct (Nat.leb_spec0 k n). now lia. easy.
+    (*erewrite unfoldTailRecStep_retT. easy.*)
+  - inv H2. edestruct IHunfolds with (fuel := S (fuel)) as (n'&eq1&?).
+    rewrite Nat.add_succ_r in eq1. 
+  induction s in P,k,a,stack|-*.
+  all:cbn.  
+Qed.*)
+  *)
+  Lemma unfoldTailRecStep_complete' a k s P s' stack res fuel:
+    unfolds H a k s s' ->
+    exists n, 
+    loopSum (n + fuel) unfoldTailRecStep  ((a,compile s++P,k)::stack,res)
+    = loopSum fuel unfoldTailRecStep ((a,P,k)::stack,rev (compile s')++res) /\ n <= L_facts.size s' *3.
+  Proof.
+    induction 1 in fuel,stack,res,P|-* using unfolds_ind'.
+    - eexists (1). cbn [loopSum unfoldTailRecStep plus compile]. cbn. 
+      destruct (Nat.leb_spec0 k n). now lia. easy.
+      (*erewrite unfoldTailRecStep_retT. easy.*)
+    - subst P0.
+      edestruct (IHunfolds []) with (fuel := S (fuel +1)) as (n'&eq1&?).
+      erewrite app_nil_r in eq1. cbn in eq1.
+      eexists (S (n' + 2)). cbn.
+      destruct (Nat.leb_spec0 k n). 2:now lia.
+      rewrite H1. cbn.  
+      replace (n' + 2 + fuel) with (n' + S (fuel + 1)) by nia.
+      rewrite eq1. replace (fuel +1) with (S fuel) by nia. cbn.
+      repeat (autorewrite with list;cbn). easy.
+    - cbn. 
+      edestruct (IHunfolds (retT :: P)) with (fuel := S fuel) as (n'&eq1&?).
+      cbn in eq1.
+      repeat (autorewrite with list;cbn).
+      rewrite <- eq1.
+      exists (S n' + 1). cbn. now rewrite <- Nat.add_assoc.  
+    - cbn. rewrite <- !app_assoc.  
+      specialize (IHunfolds2 ([appT] ++ P)) as (n2&IH2&?).  
+      specialize (IHunfolds1 (compile t ++ [appT] ++ P)) as (n1&IH1&?).
+      eexists (n1+n2+1). rewrite <- !Nat.add_assoc.
+      rewrite IH1,IH2. cbn. 
+      repeat (autorewrite with list;cbn). easy.
+  Qed.
+
+  Lemma unfoldTailRecStep_complete a k s s' n:
+    unfolds H a k s s' ->
+    L_facts.size s' * 3 + 2 <= n ->
+    loopSum n unfoldTailRecStep ([(a,(compile s),k)],[])
+    = Some (Some (rev (compile s'))).
+  Proof.
+    intros ? ?.
+    edestruct unfoldTailRecStep_complete' with (P:=@nil Tok) as (n'&eq1&?). eassumption.
+    rewrite app_nil_r in eq1.
+    eapply loopSum_mono with (n:=n'+2). now Lia.nia.
+    rewrite eq1. cbn. now rewrite  app_nil_r.
+  Qed.
+
+  (*
+  Lemma unfoldTailRecStep_sound' P a k stack acc res fuel:
+    loopSum fuel unfoldTailRecStep ((a,P,k)::stack,acc) = Some (Some res)
+    -> exists s s' fuel',
+                  P = compile s
+                  /\ unfolds H a k s s'
+                  /\ loopSum fuel unfoldTailRecStep ((a,P,k)::stack,acc)
+                    = loopSum fuel' unfoldTailRecStep (stack,rev (compile s')++acc)
+                  /\ fuel' <= fuel.
+  Proof.
+    revert P a k stack acc res.
+    induction fuel as [fuel IH] using lt_wf_ind.
+    intros ? ? ? ? ? ?.
+    destruct fuel. easy.
+    destruct P as [|[] P].
+    all:cbn in *.
+    -destruct (Nat.leb_spec0 k n) as [ |n0].
+    destruct lookup as [[R0 b]| ] eqn:eq__lookup . 2:now congruence.
+    +intros H'.
+      specialize IH with (2:=H') as (s'&fuel'&R&eq'&leq'). easy.
+      rewrite eq' in *.
+      destruct fuel' as [ |fuel']. easy.
+      cbn in *.
+      exists (lam s'), fuel'.
+      repeat apply conj.
+      1-2:now eauto using unfolds.
+      Lia.nia.
+    +intros H'.
+      do 2 eexists. repeat apply conj.
+      2,1:now eauto 10 using unfolds,not_ge.
+      Lia.nia.
+    -intros H'.
+    assert (IH':=IH).
+    specialize IH' with (2:=H') as (s1'&fuel1&R1&eq1&leq1). easy.
+    rewrite eq1 in *.
+    specialize IH with (2:=H') as (s2'&fuel2&R2&eq2&leq2). easy.
+    rewrite eq2 in *.
+    destruct fuel2 as [ |fuel2]. easy.
+    cbn in *.
+    eexists _,_. repeat apply conj.
+    1,2:now eauto using unfolds.
+    Lia.nia.
+    -intros H'.
+    specialize IH with (2:=H') as (s'&fuel'&R&eq1&leq'). easy.
+    rewrite eq1 in *.
+    destruct fuel' as [ |fuel']. easy.
+    eexists _,_. repeat apply conj.
+    1,2:now eauto using unfolds.
+    Lia.nia.
+  Qed.
+    
+  Lemma unfoldTailRecStep_sound s a k H s' fuel:
+    loopSum fuel unfoldTailRecStep ([closT (s,a) k],H,[]) = Some (Some s')
+    -> unfolds H a k s s'.
+  Proof.
+    intros H'.
+    specialize (unfoldTailRecStep_sound' H') as (k0&fuel'&R&eq'&leq').
+    rewrite eq' in *. destruct fuel'. easy.
+    inv H'. easy.
+  Qed.
+
+  Definition largestVarState : (list task * list heapEntry * list term) -> nat :=
+    fun '(stack,H,res) => max (maxl (map (fun (t:task) =>
+                                        match t with
+                                          closT q _ => largestVarC q
+                                        | _ => 0
+                                        end) stack))
+                          (max (largestVarH H) (maxl (map largestVar res))).
+
+  Lemma unfoldTailRecStep_largestVar_inv x:
+    match unfoldTailRecStep x with
+      inl x' => largestVarState x'
+    | inr (Some A)  => largestVar A
+    | _ => 0
+    end
+    <= largestVarState x.
+
+  Proof.
+    unfold unfoldTailRecStep.
+    repeat (let eq := fresh "eq" in destruct _ eqn:eq);inv eq;try congruence.
+    
+
+    
+    all:repeat match goal with
+                H : _ <=? _ = true |- _ => apply Nat.leb_le in H
+              | H : _ <=? _ = false |- _ => apply Nat.leb_gt in H
+              | H : lookup _ _ _ = Some _ |- _ => apply lookup_size in H;cbn in H
+
+              end.
+    all:unfold largestVarState,largestVarCs,largestVarC in *; cbn;fold maxl.
+    all:try Lia.lia.
+  Qed. 
+
+  Require Import Undecidability.L.Functions.Equality.
+
+
+
+  Definition unfoldBoolean H (p:clos) : option bool :=
+    let '(s,a) := p in
+    match loopSum 7 unfoldTailRecStep ([closT p 1],H,[]) with
+    | Some (Some t) =>
+      if term_eqb (lam t) (enc true)
+      then Some true
+      else if term_eqb (lam t) (enc false )
+          then Some false
+          else None       
+    | _ => None
+    end.
+
+  Lemma unfoldBoolean_complete H p (b:bool) :
+    reprC H p (enc b) -> unfoldBoolean H p = Some b.
+  Proof.
+    intros H1. inv H1. unfold unfoldBoolean.
+    erewrite unfoldTailRecStep_complete. 2:easy. 2:{ destruct b;inv H2;cbn;Lia.lia. }
+    destruct b;inv H2;cbv. all:reflexivity.
+  Qed.
+
+  Lemma unfoldBoolean_sound (H : list heapEntry) (p : clos) (b : bool) :
+    unfoldBoolean H p = Some b -> reprC H p (enc b).
+  Proof.
+    unfold unfoldBoolean.
+    destruct p as [P a]. 
+    destruct loopSum as [[]| ] eqn:H'. 2-3:easy.
+    eapply unfoldTailRecStep_sound in H'.
+    destruct (term_eqb_spec (lam t) (enc true)).
+    2: destruct (term_eqb_spec (lam t) (enc false)).
+    all:inversion 1. all:inv e. all:cbv in *. all:easy.
+  Qed.
+
+  *)
+
+End fixH.
