theories/TM/L/Compiler/Compiler_facts.v
@@ -1,13 +1,12 @@
-From Undecidability Require Import L.Datatypes.LBool L.Datatypes.Lists L.Tactics.LTactics L.Tactics.GenEncode L.Util.L_facts.
+From Undecidability Require Import L.Datatypes.LBool L.Datatypes.Lists L.Tactics.LTactics L.Util.L_facts.
 
 Require Import PslBase.FiniteTypes.FinTypes PslBase.Vectors.Vectors.
 Require Import Vector List.
 
 Require Import Undecidability.TM.Util.TM_facts.
 
-From Undecidability Require Import ProgrammingTools LM_heap_def WriteValue Copy.
-From Undecidability.L.AbstractMachines.TM_LHeapInterpreter Require Import Alphabets StepTM M_LHeapInterpreter.
-From Undecidability Require Import TM.TM L.AbstractMachines.FlatPro.LM_heap_correct.
+From Undecidability Require Import ProgrammingTools.
+From Undecidability Require Import TM.TM.
 
 From Undecidability Require Import L.L TM.TM.
 Require Import List.
@@ -15,7 +14,7 @@ Import ListNotations.
 
 Import VectorNotations.
 
-From Undecidability.LAM Require Import Compiler_spec.
+From Undecidability.TM.L.Compiler Require Import Compiler_spec.
 
 Require Import Equations.Prop.DepElim.
 
