theories/TM/L/UnfoldHeap.v
@@ -1,0 +1,68 @@
+Require Import PslBase.FiniteTypes.FinTypes PslBase.Vectors.Vectors.
+Require Import Vector List.
+
+Require Import Undecidability.TM.Util.TM_facts.
+
+From Undecidability Require Import ProgrammingTools WriteValue Copy ListTM  JumpTargetTM WriteValue.
+From Undecidability.TM.L Require Import Alphabets LookupTM.
+From Undecidability.L.AbstractMachines.FlatPro Require Import LM_heap_def LM_heap_correct.
+From Undecidability Require Import L.L TM.TM.
+Require Import List.
+Import ListNotations.
+
+
+Import VectorNotations.
+
+Require Import Equations.Prop.DepElim.
+
+
+Module UnfoldHeap.
+Section Fix.
+
+  Variable Σ : finType.
+
+  Variable retr_closures : Retract (sigList sigHClos) Σ.
+  Variable retr_heap : Retract sigHeap Σ.
+
+  Axiom retr_closures_REMOVE : Retract (sigList sigHClos) Σ.
+
+  (** Retracts *)
+  (* Closures *)
+  Local Definition retr_clos : Retract sigHClos Σ := ComposeRetract retr_closures _.
+
+  (* Closure addresses *)
+
+  Definition retr_pro_clos : Retract sigPro sigHClos := _.
+  Local Definition retr_pro : Retract sigPro Σ := ComposeRetract retr_clos retr_pro_clos.
+  Local Definition retr_tok : Retract sigCom Σ := ComposeRetract retr_pro _.
+
+  Local Definition retr_nat_clos_ad : Retract sigNat sigHClos := Retract_sigPair_X _ (Retract_id _).
+  Local Definition retr_nat_step_clos_ad : Retract sigNat Σ := ComposeRetract retr_clos retr_nat_clos_ad.
+
+  Local Definition retr_nat_clos_var : Retract sigNat sigHClos := Retract_sigPair_Y _ _.
+  Local Definition retr_nat_step_clos_var : Retract sigNat Σ := ComposeRetract retr_clos retr_nat_clos_var.
+
+  (** Instance of the [Lookup] and [JumpTarget] machine *)
+  Local Definition Step_Lookup := Lookup retr_clos retr_heap.
+
+    Variable n : nat.
+
+    Variable i_g : Fin.t n.
+    Variable i_H : Fin.t n.
+    Variable o_t : Fin.t n.
+
+    Definition M : pTM (Σ) ^+ unit n. Admitted.
+
+    Theorem Realises :
+    Realise M (fun t '(r, t') =>
+                        forall g, forall H : Heap, 
+                            t[@i_g] ≃(retr_closures_REMOVE) [g]%list (*TODO: change to clos?*) ->
+                            t[@i_H] ≃ H ->
+                            exists t,
+                            reprC H g t /\
+                            t'[@o_t] ≃(retr_pro) compile t).
+    
+    Admitted.
+
+End Fix.
+End UnfoldHeap.
